Make some proofs in Hashmap/Properties.lean and improve progress

tests/lean/Hashmap/Properties.lean
@@ -21,8 +21,9 @@ end List
 
 namespace HashMap
 
-@[pspec]
-theorem insert_in_list_spec {α : Type} (key: Usize) (value: α) (ls: List α) :
+abbrev Core.List := _root_.List
+
+theorem insert_in_list_spec0 {α : Type} (key: Usize) (value: α) (ls: List α) :
   ∃ b,
     insert_in_list α key value ls = ret b ∧
     (b ↔ List.lookup ls.v key = none)
@@ -35,7 +36,7 @@ theorem insert_in_list_spec {α : Type} (key: Usize) (value: α) (ls: List α) :
         rw [insert_in_list_loop]
         simp [h]
     else
-      have ⟨ b, hi ⟩ := insert_in_list_spec key value tl
+      have ⟨ b, hi ⟩ := insert_in_list_spec0 key value tl
       by
         exists b
         simp [insert_in_list, List.lookup]
@@ -45,7 +46,6 @@ theorem insert_in_list_spec {α : Type} (key: Usize) (value: α) (ls: List α) :
         exact hi
 
 -- Variation: use progress
-@[pspec]
 theorem insert_in_list_spec1 {α : Type} (key: Usize) (value: α) (ls: List α) :
   ∃ b,
     insert_in_list α key value ls = ret b ∧
@@ -70,7 +70,6 @@ theorem insert_in_list_spec1 {α : Type} (key: Usize) (value: α) (ls: List α) 
         simp [*, List.lookup]
 
 -- Variation: use tactics from the beginning
-@[pspec]
 theorem insert_in_list_spec2 {α : Type} (key: Usize) (value: α) (ls: List α) :
   ∃ b,
     insert_in_list α key value ls = ret b ∧
@@ -91,10 +90,10 @@ theorem insert_in_list_spec2 {α : Type} (key: Usize) (value: α) (ls: List α) 
      progress as ⟨ b h ⟩
      simp [*]
 
-@[pspec]
 theorem insert_in_list_back_spec {α : Type} (key: Usize) (value: α) (l0: List α) :
   ∃ l1,
     insert_in_list_back α key value l0 = ret l1 ∧
+    -- We update the binding
     List.lookup l1.v key = value ∧
     (∀ k, k ≠ key → List.lookup l1.v k = List.lookup l0.v k)
   := match l0 with
@@ -112,11 +111,66 @@ theorem insert_in_list_back_spec {α : Type} (key: Usize) (value: α) (l0: List 
          simp [insert_in_list_back, List.lookup]
          rw [insert_in_list_loop_back]
          simp [h, List.lookup]
-         have ⟨tl0 , _, _ ⟩ := insert_in_list_back_spec key value tl -- TODO: Use progress
-         simp [insert_in_list_back] at *
-         simp [List.lookup, *]
-         simp (config := {contextual := true}) [*]
-        
+         progress keep as heq as ⟨ tl hp1 hp2 ⟩
+         simp [insert_in_list_back] at heq
+         simp (config := {contextual := true}) [*, List.lookup]
+
+def distinct_keys (ls : Core.List (Usize × α)) := ls.pairwise_rel (λ x y => x.fst ≠ y.fst)
+
+def hash_mod_key (k : Usize) (l : Int) : Int :=
+  match hash_key k with
+  | .ret k => k.val % l
+  | _ => 0
+
+def slot_s_inv_hash (l i : Int) (ls : Core.List (Usize × α)) : Prop :=
+  ls.allP (λ (k, _) => hash_mod_key k l = i)
+
+@[simp]
+def slot_s_inv (l i : Int) (ls : Core.List (Usize × α)) : Prop :=
+  distinct_keys ls ∧
+  slot_s_inv_hash l i ls
+
+def slot_t_inv (l i : Int) (s : List α) : Prop := slot_s_inv l i s.v
+
+@[pspec]
+theorem insert_in_list_back_spec1 {α : Type} (l : Int) (key: Usize) (value: α) (l0: List α)
+  (hinv : slot_s_inv_hash l (hash_mod_key key l) l0.v) :
+  ∃ l1,
+    insert_in_list_back α key value l0 = ret l1 ∧
+    -- We update the binding
+    List.lookup l1.v key = value ∧
+    (∀ k, k ≠ key → List.lookup l1.v k = List.lookup l0.v k) ∧
+    -- We preserve part of the key invariant
+    slot_s_inv_hash l (hash_mod_key key l) l1.v
+  := match l0 with
+  | .Nil => by
+    simp [insert_in_list_back, insert_in_list_loop_back, List.lookup, List.v, slot_s_inv_hash]
+    tauto
+  | .Cons k v tl0 =>
+     if h: k = key then
+       by
+         simp [insert_in_list_back, List.lookup]
+         rw [insert_in_list_loop_back]
+         simp [h, List.lookup]
+         constructor
+         . intros; simp [*]
+         . simp [List.v, slot_s_inv_hash] at *
+           simp [*]
+     else
+       by
+         simp [insert_in_list_back, List.lookup]
+         rw [insert_in_list_loop_back]
+         simp [h, List.lookup]
+         have : slot_s_inv_hash l (hash_mod_key key l) (List.v tl0) := by
+           simp_all [List.v, slot_s_inv_hash]
+         progress keep as heq as ⟨ tl1 hp1 hp2 hp3 ⟩
+         simp only [insert_in_list_back] at heq
+         have : slot_s_inv_hash l (hash_mod_key key l) (List.v (List.Cons k v tl1)) := by
+           simp [List.v, slot_s_inv_hash] at *
+           simp [*]
+         simp (config := {contextual := true}) [*, List.lookup]
+
+
 end HashMap
 
 end hashmap
